making WHILE and OWHILE translate to slightly better CakeML

translator/std_preludeScript.sml
@@ -2,9 +2,9 @@ open HolKernel Parse boolLib bossLib; val _ = new_theory "std_prelude";
 
 open arithmeticTheory listTheory combinTheory pairTheory sumTheory;
 open optionTheory oneTheory bitTheory stringTheory whileTheory;
-open patriciaTheory finite_mapTheory pred_setTheory;
+open finite_mapTheory pred_setTheory;
 open AstTheory LibTheory AltBigStepTheory SemanticPrimitivesTheory;
-open terminationTheory;
+open terminationTheory alistTheory;
 
 open ml_translatorLib ml_translatorTheory mini_preludeTheory;;
 
@@ -148,11 +148,8 @@ val res = translate MAX_DEF;
 val res = translate EVEN_MOD2;
 val res = translate (REWRITE_RULE [EVEN_MOD2,DECIDE ``~(n = 0) = (0 < n:num)``] ODD_EVEN);
 val res = translate FUNPOW;
-val res = translate MOD_2EXP_def;
-val res = translate DIV_2EXP_def;
-val res = translate (DECIDE ``PRE n = n-1``);
 val res = translate ABS_DIFF_def;
-val res = translate DIV2_def;
+val res = translate (DECIDE ``PRE n = n-1``);
 
 (* string *)
 
@@ -197,85 +194,65 @@ val res = translate string_le_def;
 val res = translate string_gt_def;
 val res = translate string_ge_def;
 
-(* bit *)
+(* finite maps *)
 
-val res = translate bitTheory.BITS_THM2;
-val res = translate (SIMP_RULE std_ss [bitTheory.BITS_THM,DECIDE ``SUC n - n = 1``] bitTheory.BIT_def);
-val res = translate bitTheory.SBIT_def;
-
-(* patricia trees, i.e. num |-> 'a *)
-
-val FMAP_EQ_PTREE_def = Define `
-  FMAP_EQ_PTREE f p <=>
-    (FDOM f = { n | IS_SOME (PEEK p n) }) /\
-    FEVERY (\(n,x). PEEK p n = SOME x) f /\ IS_PTREE p`;
-
-val FMAP_EQ_PTREE_FLOOKUP = prove(
-  ``FMAP_EQ_PTREE f p ==> (FLOOKUP f = PEEK p)``,
-  SIMP_TAC std_ss [FUN_EQ_THM]
-  THEN SIMP_TAC std_ss [FMAP_EQ_PTREE_def,PEEK_ADD,FAPPLY_FUPDATE_THM,
-    FDOM_FUPDATE,FEVERY_DEF,IN_INSERT,EXTENSION,FLOOKUP_DEF,GSPECIFICATION]
-  THEN REPEAT STRIP_TAC THEN Cases_on `p ' x`
-  THEN METIS_TAC [IS_SOME_DEF,SOME_11]);
-
-val FMAP_EQ_PTREE_FUPDATE = prove(
-  ``FMAP_EQ_PTREE f p ==>
-    FMAP_EQ_PTREE (FUPDATE f (n,x)) (ADD p (n,x))``,
-  SIMP_TAC std_ss [FMAP_EQ_PTREE_def,PEEK_ADD,FAPPLY_FUPDATE_THM,
-    FDOM_FUPDATE,FEVERY_DEF,IN_INSERT,GSPECIFICATION,EXTENSION,ADD_IS_PTREE]
-  THEN REPEAT STRIP_TAC THEN Cases_on `x' = n` THEN FULL_SIMP_TAC std_ss []);
-
-val FMAP_EQ_PTREE_DOMSUB = prove(
-  ``FMAP_EQ_PTREE f p ==>
-    FMAP_EQ_PTREE (f \\ n) (REMOVE p n)``,
-  SIMP_TAC (srw_ss()) [FMAP_EQ_PTREE_def,FEVERY_DEF,PEEK_def,
-    IN_INSERT,GSPECIFICATION,EXTENSION,DOMSUB_FAPPLY,PEEK_REMOVE]
-  THEN REPEAT STRIP_TAC THEN Cases_on `x = n`
-  THEN FULL_SIMP_TAC std_ss [DOMSUB_FAPPLY_NEQ]);
-
-val _ = register_type ``:'a ptree``;
-val PTREE_TYPE_def = fetch "-" "PTREE_TYPE_def";
+val FMAP_EQ_ALIST_def = Define `
+  FMAP_EQ_ALIST f l <=> (ALOOKUP l = FLOOKUP f)`;
 
 val FMAP_TYPE_def = Define `
-  FMAP_TYPE a f = \v. ?p. PTREE_TYPE a p v /\ FMAP_EQ_PTREE f p`;
+  FMAP_TYPE (a:'a -> v -> bool) (b:'b -> v -> bool) (f:'a|->'b) =
+    \v. ?l. LIST_TYPE (PAIR_TYPE a b) l v /\ FMAP_EQ_ALIST f l`;
 
-val _ = add_type_inv ``FMAP_TYPE (a:'a -> v -> bool)`` ``:'a ptree``;
+val _ = add_type_inv ``FMAP_TYPE (a:'a -> v -> bool) (b:'b -> v -> bool)``
+                     ``:('a # 'b) list``;
 
-val res = translate BRANCHING_BIT_def;
-val PEEK_eval = translate PEEK_def;
+val ALOOKUP_eval = translate ALOOKUP_def;
 
 val Eval_FLOOKUP = prove(
-  ``!v. ((PTREE_TYPE a --> NUM --> OPTION_TYPE a) PEEK) v ==>
-        ((FMAP_TYPE a --> NUM --> OPTION_TYPE a) FLOOKUP) v``,
+  ``!v. ((LIST_TYPE (PAIR_TYPE (b:'b -> v -> bool) (a:'a -> v -> bool)) -->
+          b --> OPTION_TYPE a) ALOOKUP) v ==>
+        ((FMAP_TYPE b a --> b --> OPTION_TYPE a) FLOOKUP) v``,
   SIMP_TAC (srw_ss()) [Arrow_def,AppReturns_def,FMAP_TYPE_def,
-    PULL_EXISTS] THEN METIS_TAC [FMAP_EQ_PTREE_FLOOKUP])
-  |> MATCH_MP (MATCH_MP Eval_WEAKEN PEEK_eval)
+    PULL_EXISTS,FMAP_EQ_ALIST_def] THEN METIS_TAC [])
+  |> MATCH_MP (MATCH_MP Eval_WEAKEN ALOOKUP_eval)
   |> store_eval_thm;
 
-val res = translate MOD_2EXP_EQ_def;
-val res = translate JOIN_def;
-val ADD_eval = translate ADD_def;
+val AUPDATE_def = Define `AUPDATE l (x:'a,y:'b) = (x,y)::l`;
+val AUPDATE_eval = translate AUPDATE_def;
+
+val FMAP_EQ_ALIST_UPDATE = prove(
+  ``FMAP_EQ_ALIST f l ==> FMAP_EQ_ALIST (FUPDATE f (x,y)) (AUPDATE l (x,y))``,
+  SIMP_TAC (srw_ss()) [FMAP_EQ_ALIST_def,AUPDATE_def,ALOOKUP_def,FUN_EQ_THM,
+    finite_mapTheory.FLOOKUP_DEF,finite_mapTheory.FAPPLY_FUPDATE_THM]
+  THEN METIS_TAC []);
 
 val Eval_FUPDATE = prove(
-  ``!v. ((PTREE_TYPE a --> PAIR_TYPE NUM a --> PTREE_TYPE a) ADD) v ==>
-        ((FMAP_TYPE a --> PAIR_TYPE NUM a --> FMAP_TYPE a) FUPDATE) v``,
-  SIMP_TAC (srw_ss()) [Arrow_def,AppReturns_def,FMAP_TYPE_def]
-  THEN METIS_TAC [FMAP_EQ_PTREE_FUPDATE,PAIR])
-  |> MATCH_MP (MATCH_MP Eval_WEAKEN ADD_eval)
+  ``!v. ((LIST_TYPE (PAIR_TYPE a b) -->
+          PAIR_TYPE (a:'a -> v -> bool) (b:'b -> v -> bool) -->
+          LIST_TYPE (PAIR_TYPE a b)) AUPDATE) v ==>
+        ((FMAP_TYPE a b --> PAIR_TYPE a b --> FMAP_TYPE a b) FUPDATE) v``,
+  SIMP_TAC (srw_ss()) [Arrow_def,AppReturns_def,FMAP_TYPE_def,
+    PULL_EXISTS] THEN REPEAT STRIP_TAC THEN RES_TAC
+  THEN Q.EXISTS_TAC `u` THEN FULL_SIMP_TAC std_ss []
+  THEN REPEAT STRIP_TAC THEN RES_TAC
+  THEN Q.LIST_EXISTS_TAC [`u'`,`AUPDATE l x'`]
+  THEN FULL_SIMP_TAC std_ss [] THEN METIS_TAC [FMAP_EQ_ALIST_UPDATE,PAIR])
+  |> MATCH_MP (MATCH_MP Eval_WEAKEN AUPDATE_eval)
   |> store_eval_thm;
 
-val res = translate BRANCH_def;
-val REMOVE_eval = translate REMOVE_def;
+val NIL_eval = hol2deep ``[]:('a # 'b) list``
 
-val Eval_DOMSUB = prove(
-  ``!v. ((PTREE_TYPE a --> NUM --> PTREE_TYPE a) REMOVE) v ==>
-        ((FMAP_TYPE a --> NUM --> FMAP_TYPE a) $\\) v``,
-  SIMP_TAC (srw_ss()) [Arrow_def,AppReturns_def,FMAP_TYPE_def]
-  THEN METIS_TAC [FMAP_EQ_PTREE_DOMSUB,PAIR])
-  |> MATCH_MP (MATCH_MP Eval_WEAKEN REMOVE_eval)
+val Eval_FEMPTY = prove(
+  ``!v. (LIST_TYPE (PAIR_TYPE (a:'a -> v -> bool) (b:'b -> v -> bool)) []) v ==>
+        ((FMAP_TYPE a b) FEMPTY) v``,
+  SIMP_TAC (srw_ss()) [Arrow_def,AppReturns_def,FMAP_TYPE_def,
+    PULL_EXISTS,FMAP_EQ_ALIST_def] THEN REPEAT STRIP_TAC THEN Q.EXISTS_TAC `[]`
+  THEN FULL_SIMP_TAC (srw_ss()) [ALOOKUP_def,FUN_EQ_THM,
+         finite_mapTheory.FLOOKUP_DEF])
+  |> MATCH_MP (MATCH_MP Eval_WEAKEN NIL_eval)
   |> store_eval_thm;
 
-(* while and owhile *)
+(* while, owhile and least *)
 
 val IS_SOME_OWHILE_THM = prove(
   ``!g f x. (IS_SOME (OWHILE g f x)) =
@@ -297,112 +274,105 @@ val evaluate_closure_INTRO = prove(
 
 val EXISTS_SWAP = METIS_PROVE [] ``(?x y. P x y) ==> (?y x. P x y)``
 
-(* val _ = augment_srw_ss [rewrites [do_tapp_def]]; *)
-
 val tac =
   REPEAT STRIP_TAC
   THEN FULL_SIMP_TAC std_ss [PRECONDITION_def,IS_SOME_OWHILE_THM,Eval_def]
   THEN SIMP_TAC (srw_ss()) [Once evaluate'_cases,build_rec_env_def]
+  THEN SIMP_TAC (srw_ss()) [Once Arrow_def,AppReturns_def]
+  THEN SIMP_TAC (srw_ss()) [evaluate_closure_def,do_app_def,
+                            find_recfun_def,bind_def,build_rec_env_def]
+  THEN SIMP_TAC std_ss [Once Eq_def]
+  THEN NTAC 2 STRIP_TAC
+  THEN SIMP_TAC (srw_ss()) [Once evaluate'_cases,build_rec_env_def]
+  THEN SIMP_TAC (srw_ss()) [Once Arrow_def,AppReturns_def]
+  THEN SIMP_TAC (srw_ss()) [evaluate_closure_def,do_app_def,
+                            find_recfun_def,bind_def,build_rec_env_def]
+  THEN SIMP_TAC std_ss [Once Eq_def]
+  THEN NTAC 2 STRIP_TAC
+  THEN SIMP_TAC (srw_ss()) [Once evaluate'_cases,build_rec_env_def]
+  THEN Q.ABBREV_TAC `gv = v'` THEN Q.ABBREV_TAC `fv = v''`
+  THEN POP_ASSUM (K ALL_TAC) THEN POP_ASSUM (K ALL_TAC)
   THEN SIMP_TAC (srw_ss()) [Once evaluate'_cases,build_rec_env_def]
   THEN SIMP_TAC (srw_ss()) [lookup_def,bind_def]
   THEN SIMP_TAC (srw_ss()) [Once Arrow_def,AppReturns_def]
-  THEN SIMP_TAC (srw_ss()) [evaluate_closure_def,do_app_def,find_recfun_def,bind_def,build_rec_env_def]
-  THEN SIMP_TAC (srw_ss()) [Once evaluate'_cases]
-  THEN SIMP_TAC (srw_ss()) [Once Arrow_def,AppReturns_def]
-  THEN SIMP_TAC (srw_ss()) [evaluate_closure_def,do_app_def,bind_def]
-  THEN SIMP_TAC (srw_ss()) [Once evaluate'_cases]
-  THEN SIMP_TAC std_ss [Once Eq_def] THEN SIMP_TAC std_ss [Once Eq_def]
-  THEN REPEAT STRIP_TAC
-  THEN SIMP_TAC (srw_ss()) [Once Arrow_def,AppReturns_def]
-  THEN SIMP_TAC (srw_ss()) [evaluate_closure_def,do_app_def,bind_def]
   THEN SIMP_TAC std_ss [Once Eq_def] THEN REPEAT STRIP_TAC
+  THEN SIMP_TAC (srw_ss()) [evaluate_closure_def,do_app_def,
+                            find_recfun_def,bind_def,build_rec_env_def]
+  THEN Q.ABBREV_TAC `xv = v'` THEN POP_ASSUM (K ALL_TAC)
   THEN REPEAT (POP_ASSUM MP_TAC)
-  THEN Q.SPEC_TAC (`x`,`x`)
-  THEN Q.SPEC_TAC (`v'`,`v1`)
-  THEN Q.SPEC_TAC (`v''`,`v2`)
-  THEN Q.SPEC_TAC (`v'''`,`v3`)
-  THEN Q.SPEC_TAC (`f`,`f`)
-  THEN Q.SPEC_TAC (`g`,`g`)
-  THEN FULL_SIMP_TAC std_ss [GSYM Eval_def] THEN CONV_TAC (DEPTH_CONV ETA_CONV)
+  THEN Q.SPEC_TAC (`x`,`x`) THEN Q.SPEC_TAC (`xv`,`xv`)
+  THEN SIMP_TAC std_ss [GSYM Eval_def]
+  THEN CONV_TAC (DEPTH_CONV ETA_CONV)
   THEN Induct_on `n` THEN1
    (FULL_SIMP_TAC std_ss [FUNPOW] THEN REPEAT STRIP_TAC
     THEN ONCE_REWRITE_TAC [OWHILE_THM,WHILE]
     THEN MATCH_MP_TAC (REWRITE_RULE [AND_IMP_INTRO] Eval_If |> GEN_ALL)
     THEN Q.LIST_EXISTS_TAC [`T`,`F`,`T`]
     THEN FULL_SIMP_TAC std_ss [CONTAINER_def]
-    THEN REPEAT STRIP_TAC THEN1
-     (`g x = F` by ALL_TAC
-      THEN1 (FULL_SIMP_TAC std_ss [])
-      THEN POP_ASSUM (fn th => ONCE_REWRITE_TAC [GSYM th])
-      THEN MATCH_MP_TAC (REWRITE_RULE [AND_IMP_INTRO] Eval_Arrow)
-      THEN ASM_SIMP_TAC (srw_ss()) [Once evaluate'_cases,lookup_def,Eval_def]
-      THEN ASM_SIMP_TAC (srw_ss()) [Once evaluate'_cases,lookup_def,Eval_def])
-    THEN NTAC 6 (ASM_SIMP_TAC (srw_ss()) [Once evaluate'_cases,lookup_def,
-         EVAL ``OPTION_TYPE a (SOME x) v``,Eval_def,do_app_def]))
+    THEN REVERSE STRIP_TAC THEN1
+      (NTAC 6 (ASM_SIMP_TAC (srw_ss()) [Once evaluate'_cases,lookup_def,
+                 EVAL ``OPTION_TYPE a (SOME x) v``,Eval_def,do_app_def]))
+    THEN `F = g x` by METIS_TAC []
+    THEN POP_ASSUM (fn th => ONCE_REWRITE_TAC [th])
+    THEN MATCH_MP_TAC (REWRITE_RULE [AND_IMP_INTRO] Eval_Arrow)
+    THEN ASM_SIMP_TAC (srw_ss()) [Once evaluate'_cases,lookup_def,Eval_def]
+    THEN ASM_SIMP_TAC (srw_ss()) [Once evaluate'_cases,lookup_def,Eval_def])
   THEN FULL_SIMP_TAC std_ss [FUNPOW] THEN REPEAT STRIP_TAC
   THEN ONCE_REWRITE_TAC [OWHILE_THM,WHILE]
   THEN MATCH_MP_TAC (REWRITE_RULE [AND_IMP_INTRO] Eval_If |> GEN_ALL)
   THEN Q.LIST_EXISTS_TAC [`F`,`T`,`T`]
-  THEN FULL_SIMP_TAC std_ss [CONTAINER_def]
-  THEN `0 < SUC n` by DECIDE_TAC THEN RES_TAC
-  THEN REVERSE STRIP_TAC THEN1 FULL_SIMP_TAC std_ss [FUNPOW]
+  THEN `g x` by
+   (Q.PAT_ASSUM `!m.bbb` (MP_TAC o Q.SPEC `0`) THEN FULL_SIMP_TAC std_ss [FUNPOW])
+  THEN ASM_SIMP_TAC std_ss [CONTAINER_def]
   THEN STRIP_TAC THEN1
-   (MATCH_MP_TAC (REWRITE_RULE [AND_IMP_INTRO] Eval_Arrow)
+   (`T = g x` by FULL_SIMP_TAC std_ss []
+    THEN POP_ASSUM (fn th => ONCE_REWRITE_TAC [th])
+    THEN MATCH_MP_TAC (REWRITE_RULE [AND_IMP_INTRO] Eval_Arrow)
     THEN ASM_SIMP_TAC (srw_ss()) [Once evaluate'_cases,lookup_def,Eval_def]
     THEN ASM_SIMP_TAC (srw_ss()) [Once evaluate'_cases,lookup_def,Eval_def])
   THEN ASM_SIMP_TAC (srw_ss()) [Once evaluate'_cases,lookup_def,Eval_def]
+  THEN ONCE_REWRITE_TAC [evaluate'_empty_store] THEN FULL_SIMP_TAC std_ss []
+  THEN ONCE_REWRITE_TAC [do_app_empty_store] THEN FULL_SIMP_TAC std_ss []
+  THEN ONCE_REWRITE_TAC [evaluate'_empty_store] THEN FULL_SIMP_TAC std_ss []
   THEN ASM_SIMP_TAC (srw_ss()) [Once evaluate'_cases,lookup_def,Eval_def]
-  THEN ASM_SIMP_TAC (srw_ss()) [Once evaluate'_cases,lookup_def,Eval_def]
-  THEN ASM_SIMP_TAC (srw_ss()) [Once evaluate'_cases,lookup_def,Eval_def]
-  THEN ASM_SIMP_TAC (srw_ss()) [Once evaluate'_cases,lookup_def,Eval_def]
-  THEN SIMP_TAC (srw_ss()) [Once do_app_def,find_recfun_def]
-  THEN ASM_SIMP_TAC (srw_ss()) [Once evaluate'_cases,lookup_def,Eval_def]
-  THEN ASM_SIMP_TAC (srw_ss()) [Once evaluate'_cases,lookup_def,Eval_def]
-  THEN SIMP_TAC (srw_ss()) [Once do_app_def,find_recfun_def]
-  THEN ASM_SIMP_TAC (srw_ss()) [Once evaluate'_cases,lookup_def,Eval_def]
-  THEN SIMP_TAC (srw_ss()) [Once do_app_def,find_recfun_def]
   THEN ASM_SIMP_TAC (srw_ss()) [Once evaluate'_cases,lookup_def,Eval_def]
   THEN ASM_SIMP_TAC (srw_ss()) [Once evaluate'_cases,lookup_def,Eval_def]
   THEN ASM_SIMP_TAC (srw_ss()) [Once evaluate'_cases,lookup_def,Eval_def]
   THEN ONCE_REWRITE_TAC [evaluate'_empty_store] THEN FULL_SIMP_TAC std_ss []
-  THEN ONCE_REWRITE_TAC [evaluate'_empty_store] THEN FULL_SIMP_TAC std_ss []
-  THEN FULL_SIMP_TAC std_ss [evaluate_closure_INTRO]
+  THEN SIMP_TAC std_ss [evaluate_closure_INTRO]
+  THEN FULL_SIMP_TAC (srw_ss()) [do_app_def,find_recfun_def,
+         bind_def,build_rec_env_def]
   THEN FULL_SIMP_TAC std_ss [PULL_EXISTS,PULL_FORALL]
   THEN HO_MATCH_MP_TAC EXISTS_SWAP
-  THEN `?v_fx. evaluate_closure v3 v2 v_fx /\ a (f x) v_fx` by ALL_TAC THEN1
+  THEN `?v_fx. evaluate_closure xv fv v_fx /\ a (f x) v_fx` by ALL_TAC THEN1
        (FULL_SIMP_TAC std_ss [Arrow_def,AppReturns_def] THEN METIS_TAC [])
   THEN Q.EXISTS_TAC `v_fx` THEN FULL_SIMP_TAC std_ss [GSYM Eval_def]
   THEN FULL_SIMP_TAC std_ss [AND_IMP_INTRO] THEN CONV_TAC (DEPTH_CONV ETA_CONV)
-  THEN SIMP_TAC (srw_ss()) [bind_def,build_rec_env_def]
   THEN Q.PAT_ASSUM `!x1 x2. bbb` MATCH_MP_TAC THEN ASM_SIMP_TAC std_ss []
   THEN REPEAT STRIP_TAC
   THEN Q.PAT_ASSUM `!m. bbb` (MP_TAC o Q.SPEC `SUC m`)
   THEN FULL_SIMP_TAC (srw_ss()) [FUNPOW]
 
-val Eval_OWHILE = prove(
-  ``PRECONDITION (IS_SOME (OWHILE g f (x:'a))) ==>
-    Eval env (Letrec
-      [("owhile","g",
-        Fun "f" (Fun "x"
-          (If (App Opapp (Var (Short "g")) (Var (Short "x")))
-            (App Opapp
-             (App Opapp (App Opapp (Var (Short "owhile")) (Var (Short "g")))
-              (Var (Short "f"))) (App Opapp (Var (Short "f")) (Var (Short "x"))))
-            (Con (Short "Some") [Var (Short "x")]))))] (Var (Short "owhile")))
-      ((Eq (a --> BOOL) g --> Eq (a --> a) f --> Eq a x --> OPTION_TYPE a) OWHILE)``,
-  tac) |> UNDISCH_ALL |> store_eval_thm;
-
 val Eval_WHILE = prove(
   ``PRECONDITION (IS_SOME (OWHILE g f (x:'a))) ==>
-    Eval env (Letrec
-         [("w","g",
-           Fun "f" (Fun "x"
-            (If (App Opapp (Var (Short "g")) (Var (Short "x")))
-               (App Opapp
-                (App Opapp (App Opapp (Var (Short "w")) (Var (Short "g")))
-                 (Var (Short "f"))) (App Opapp (Var (Short "f")) (Var (Short "x"))))
-               (Var (Short "x")))))] (Var (Short "w")))
+    Eval env (Fun "g" (Fun "f" (Letrec
+         [("w","x",
+             (If (App Opapp (Var (Short "g")) (Var (Short "x")))
+                 (App Opapp (Var (Short "w"))
+                   (App Opapp (Var (Short "f")) (Var (Short "x"))))
+               (Var (Short "x"))))] (Var (Short "w")))))
       ((Eq (a --> BOOL) g --> Eq (a --> a) f --> Eq a x --> a) WHILE)``,
+  tac) |> UNDISCH_ALL |> store_eval_thm;
+
+val Eval_OWHILE = prove(
+  ``PRECONDITION (IS_SOME (OWHILE g f (x:'a))) ==>
+    Eval env (Fun "g" (Fun "f" (Letrec
+         [("w","x",
+             (If (App Opapp (Var (Short "g")) (Var (Short "x")))
+                 (App Opapp (Var (Short "w"))
+                   (App Opapp (Var (Short "f")) (Var (Short "x"))))
+               (Con (Short "Some") [Var (Short "x")])))] (Var (Short "w")))))
+      ((Eq (a --> BOOL) g --> Eq (a --> a) f --> Eq a x --> OPTION_TYPE a) OWHILE)``,
   tac) |> UNDISCH_ALL |> store_eval_thm;
 
 val SUC_LEMMA = prove(``SUC = \x. x+1``,SIMP_TAC std_ss [FUN_EQ_THM,ADD1]);
